generalize bblock_equiv into bblock_simu (abstract_bb)

mppa_k1c/abstractbb/Impure/ocaml/ImpIOOracles.ml
@@ -53,14 +53,6 @@ let memo_int2pos: int -> int -> BinNums.positive
           Hashtbl.add t i pi;
           pi
      in find;;
-           
-(* 
-let string_coq2caml: char list -> string
-  = fun l ->
-    let buf = Buffer.create (List.length l) in
-    List.iter (fun c -> Buffer.add_char buf c) l;
-    Buffer.contents buf;;
-*)
 
 let new_exit_observer: (unit -> unit) -> (unit -> unit) ref
   = fun f ->
@@ -123,8 +115,8 @@ let zTr: BinNums.coq_Z -> int
 let ten = BinNums.Zpos (BinNums.Coq_xO (BinNums.Coq_xI (BinNums.Coq_xO BinNums.Coq_xH)))
 
 let rec string_of_pos (p:BinNums.positive) (acc: pstring): pstring
-= let (q,r) = BinInt.Z.pos_div_eucl p ten in       
-  let acc0 = Concat (CamlStr (string_of_int (zTr r)), acc) in    
+= let (q,r) = BinInt.Z.pos_div_eucl p ten in
+  let acc0 = Concat (CamlStr (string_of_int (zTr r)), acc) in
   match q with
   | BinNums.Z0 -> acc0
   | BinNums.Zpos p0 -> string_of_pos p0 acc0
@@ -134,7 +126,7 @@ let rec string_of_pos (p:BinNums.positive) (acc: pstring): pstring
 let string_of_Z_debug: BinNums.coq_Z -> pstring
 = fun p -> CamlStr (string_of_int (zTr p))
 *)
-     
+
 let string_of_Z: BinNums.coq_Z -> pstring
 = function
   | BinNums.Z0 -> CamlStr "0"
@@ -148,4 +140,3 @@ let timer ((f:'a -> 'b), (x:'a)) : 'b =
   let rt = (Unix.times()).Unix.tms_utime -. itime in
   Printf.printf "time = %f\n" rt;
   r
-    
